Goal normalization proof and cleanup

Goal_Normalization.thy
@@ -1,6 +1,7 @@
 theory Goal_Normalization
 imports "AI_Planning_Languages_Semantics.PDDL_STRIPS_Semantics"
-    String_Shenanigans Utils PDDL_Sema_Supplement DNF
+    PDDL_Sema_Supplement PDDL_Instance_Relationships
+    String_Shenanigans Utils DNF
 begin
 
 context ast_domain begin
@@ -18,11 +19,9 @@ context ast_domain begin
     Action_Schema goal_ac_name [] g goal_effect"
 end
 
-definition "obj_to_term obj \<equiv> term.VAR obj"
-
 context ast_problem begin
 
-  definition "term_goal \<equiv> (map_formula\<circ>map_atom) term.CONST (goal P)"
+  definition "term_goal \<equiv> map_atom_fmla term.CONST (goal P)"
   
   definition "degoal_dom \<equiv>
     Domain
@@ -88,7 +87,6 @@ subsection \<open>Well-Formedness\<close>
 
 context wf_ast_problem3 begin
 
-
 lemma pred_stack: "Pred ` predicate.name ` ps = ps" by force
 
 lemma g_preds_dist: "distinct (map pred (predicates D3))"
@@ -130,9 +128,6 @@ proof -
   thus ?thesis using degoal_dom_sel wf_D(6) by auto
 qed
 
-thm wf_action_schema.simps
-thm wf_action_schema_alt
-
 lemma g_sig:
   assumes "sig p = Some xs" shows "d3.sig p = Some xs"
 proof -
@@ -142,25 +137,29 @@ proof -
     using ast_domain.pred_resolve by blast
 qed
 
-lemma g_fmla_wf:
-  assumes "wf_fmla tyt \<phi>" shows "d3.wf_fmla tyt \<phi>"
-  using assms
-proof (induction \<phi>)
-  case (Atom x) thus ?case
-  proof (cases x)
-    case (predAtm p xs)
-    hence a: "wf_pred_atom tyt (p, xs)" using assms Atom by simp
-    then obtain Ts where sig: "sig p = Some Ts"
-      by fastforce
-    with a have "list_all2 (is_of_type tyt) xs Ts" by simp
-    hence "list_all2 (d3.is_of_type tyt) xs Ts"
-      unfolding ast_domain.is_of_type_def ast_domain.of_type_def ast_domain.subtype_rel_def degoal_dom_sel(1)
-      by simp
-    moreover have "d3.sig p = Some Ts" using g_sig sig by simp
-    ultimately have "d3.wf_pred_atom tyt (p, xs)" by simp
-    then show ?thesis using predAtm by simp
-  qed simp
-qed auto
+lemma g_is_of_type: "is_of_type = d3.is_of_type"
+  apply (rule ext)
+  unfolding ast_domain.is_of_type_def ast_domain.of_type_def ast_domain.subtype_rel_def degoal_dom_sel(1)
+  by simp
+
+lemma g_atom_wf:
+  assumes "wf_atom tyt a" shows "d3.wf_atom tyt a"
+using assms proof (cases a)
+  case [simp]: (predAtm p xs)
+  hence a: "wf_pred_atom tyt (p, xs)" using assms by simp
+  then obtain Ts where sig: "sig p = Some Ts" by fastforce
+  with a have "list_all2 (is_of_type tyt) xs Ts" by simp
+  hence "list_all2 (d3.is_of_type tyt) xs Ts" using g_is_of_type by metis
+  moreover have "d3.sig p = Some Ts" using g_sig sig by simp
+  ultimately have "d3.wf_pred_atom tyt (p, xs)" by simp
+  then show ?thesis using predAtm by simp
+qed simp
+
+lemma g_fmla_wf: "wf_fmla tyt \<phi> \<Longrightarrow> d3.wf_fmla tyt \<phi>"
+  using g_atom_wf co_fmla_wf by blast
+
+lemma g_eff_wf: "wf_effect tyt \<epsilon> \<Longrightarrow> d3.wf_effect tyt \<epsilon>"
+  using g_atom_wf co_effect_wf by blast
 
 lemma g_constT:
   "objT = d3.constT"
@@ -171,63 +170,42 @@ lemma g_objT:
   "objT = p3.objT"
   using g_constT d3.constT_def p3.objT_def degoal_prob_sel by simp
 
-lemma g_eff_wf:
-  assumes "wf_effect tyt \<epsilon>" shows "d3.wf_effect tyt \<epsilon>"
-  using assms apply (cases \<epsilon>; simp)
-  using ast_domain.wf_fmla_atom_alt g_fmla_wf by blast
+lemma g_wm_wf: "wf_world_model wm \<Longrightarrow> p3.wf_world_model wm"
+  using degoal_prob_sel(1) g_objT g_atom_wf co_wm_wf by metis
 
-lemma g_wm_wf:
-  assumes "wf_world_model wm" shows "p3.wf_world_model wm"
-  using assms ast_problem.wf_world_model_def ast_domain.wf_fmla_atom_alt
-    degoal_prob_sel(1) g_fmla_wf g_objT by metis
+lemma g_obj_of_type: "is_obj_of_type = p3.is_obj_of_type"
+  unfolding ast_problem.is_obj_of_type_alt ast_domain.is_of_type_def ast_domain.of_type_def
+    ast_domain.subtype_rel_def
+  using g_objT degoal_dom_sel(1) degoal_prob_sel(1) by metis
 
-lemma wf_fmla_mono:
-  assumes "tys \<subseteq>\<^sub>m tys'" "wf_fmla tys \<phi>"
-  shows "wf_fmla tys' \<phi>"
-  using assms apply (induction \<phi>)
-  apply (simp add: wf_atom_mono) by simp_all
-
-lemma wf_eff_mono:
-  assumes "tys \<subseteq>\<^sub>m tys'" "wf_effect tys eff"
-  shows "wf_effect tys' eff"
-  using assms apply (cases eff)
-  using wf_fmla_atom_mono by auto
+lemma is_of_type_term: "is_of_type tyt x t \<longleftrightarrow> is_of_type (ty_term xd tyt) (term.CONST x) t"
+  unfolding is_of_type_def by simp
 
 lemma wf_atom_to_term:
   assumes "wf_atom tyt a"
-  shows "wf_atom (ty_term xd tyt) (map_atom term.CONST a)"
+  shows "wf_atom (ty_term vart tyt) (map_atom term.CONST a)"
 proof (cases a)
-  case (predAtm p xs)
-  with assms obtain Ts where sig: "sig p = Some Ts" by fastforce
-  from sig have match: "list_all2 (is_of_type tyt) xs Ts" using predAtm assms by simp
-
-  have "list_all2 (is_of_type (ty_term xd tyt)) (map term.CONST xs) Ts"
-    using match
-  proof (induction xs arbitrary: Ts)
-    case (Cons g gs)
-    then obtain t ts where ts: "t # ts = Ts"
-      by (metis list_all2_Cons1)
-    with Cons have 1: "is_of_type tyt g t" "list_all2 (is_of_type tyt) gs ts"
-      by auto
-    hence "list_all2 (is_of_type (ty_term xd tyt)) (map term.CONST gs) ts"
-      "is_of_type (ty_term xd tyt) (term.CONST g) t"
-      using Cons.IH apply simp
-      using 1 by (simp add: ast_domain.is_of_type_def)
-    thus ?case using ts list_all2_Cons1 by auto
+  case [simp]: (predAtm p xs)
+  with assms obtain Ts where [simp]: "sig p = Some Ts" by fastforce
+  hence match: "list_all2 (is_of_type tyt) xs Ts" using assms by simp
+  hence "list_all2 (is_of_type (ty_term vart tyt)) (map term.CONST xs) Ts"
+  using match proof (induction xs Ts) (* rule: list_all2_induct *)
+    case Cons thus ?case using is_of_type_term list_all2_Cons by simp
   qed simp
 
-  thus ?thesis using predAtm sig by simp
+  thus ?thesis by simp
 next
   case Eq thus ?thesis using assms by auto
 qed
 
 lemma wf_fmla_to_term:
   assumes "wf_fmla tyt F"
-  shows "wf_fmla (ty_term xd tyt) (map_atom_fmla term.CONST F)"
+  shows "wf_fmla (ty_term vart tyt) (map_atom_fmla term.CONST F)"
   using assms by (induction F) (simp_all add: wf_atom_to_term)
 
 lemma g_acs_wf: "(\<forall>a\<in>set (actions D3). d3.wf_action_schema a)"
 proof -
+  (* carrying over original actinos *)
   have 1: "d3.wf_action_schema ac" if "wf_action_schema ac" for ac
   proof (cases ac)
     case (Action_Schema n params pre eff)
@@ -235,7 +213,7 @@ proof -
     let ?tyt = "ty_term (map_of params) constT"
     let ?tyt3 = "ty_term (map_of params) d3.constT"
     have tyts: "?tyt \<subseteq>\<^sub>m ?tyt3"
-      using degoal_dom_sel ast_domain.constT_def g_constT constT_ss_objT
+      using ast_domain.constT_def g_constT constT_ss_objT
       by (simp add: ty_term_mono)
 
     from that have "wf_fmla ?tyt pre \<and> wf_effect ?tyt eff"
@@ -246,6 +224,7 @@ proof -
     ultimately show ?thesis using Action_Schema ast_domain.wf_action_schema.simps by simp
   qed
 
+  (* goal action well-formed *)
   let ?gac = "goal_ac term_goal"
   have "d3.wf_action_schema ?gac"
   proof -
@@ -256,18 +235,17 @@ proof -
       unfolding term_goal_def
       using wf_P g_constT wf_fmla_to_term g_fmla_wf by metis
     have 3: "d3.wf_effect ?tyt goal_effect"
-      (* d_preds_dist not needed, since goal_pred is the first in the list *)
-      using degoal_dom_sel(2) d3.sig_def goal_pred_decl_def by force
+      (* g_preds_dist not needed, since goal_pred is the first in the list *)
+      using d3.sig_def goal_pred_decl_def by force
     from 1 2 3 show ?thesis
       by (simp add: goal_ac_def)
 
   qed
-  with 1 show ?thesis using wf_D(7) degoal_dom_sel by simp
+  with 1 show ?thesis using wf_D(7) by simp
 qed
 
 lemma degoal_dom_wf: "d3.wf_domain"
 proof -
-  note degoal_dom_sel[simp]
   have c1: "d3.wf_types" using ast_domain.wf_types_def wf_D by simp
   note c2 = g_preds_dist
   note c3 = g_preds_wf
@@ -280,7 +258,6 @@ qed
 
 lemma degoal_prob_wf: "p3.wf_problem"
 proof -
-  note degoal_prob_sel[simp] degoal_dom_sel[simp]
   note c1 = degoal_dom_wf
   have c2: "distinct (map fst (objects degoal_prob) @ map fst (consts p3.D))"
     using wf_D wf_P by simp
@@ -288,7 +265,7 @@ proof -
   note c4 = wf_P(3)
   have c5: "p3.wf_world_model (set (init P))" using g_wm_wf wf_P(4) by simp
   have c6: "p3.wf_fmla p3.objT (goal degoal_prob)"
-    (* d_preds_dist not needed, since goal_pred is the first in the list *)
+    (* g_preds_dist not needed, since goal_pred is the first in the list *)
     using d3.sig_def goal_pred_decl_def by auto
   from c1 c2 c3 c4 c5 c6 show ?thesis using p3.wf_problem_def by simp
 qed
@@ -303,41 +280,40 @@ sublocale wf_ast_problem3 \<subseteq> p3: wf_ast_problem P3
 
 context wf_ast_problem3 begin
 
-lemma resolve_ac_g:
+lemma resolve_goal_ac:
   "p3.resolve_action_schema goal_ac_name = Some (goal_ac term_goal)"
   using goal_ac_def p3.res_aux degoal_prob_sel degoal_dom_sel by simp
 
-lemma wf_pa_g:
+lemma wf_goal_pa:
   "p3.wf_plan_action \<pi>\<^sub>g"
 proof -
   have "p3.action_params_match (goal_ac term_goal) []"
     unfolding goal_ac_def p3.action_params_match_def by simp
-  with resolve_ac_g show ?thesis using p3.wf_plan_action_simple by fastforce
+  with resolve_goal_ac show ?thesis using p3.wf_plan_action_simple by fastforce
 qed
-
-term "(map_formula\<circ>map_atom) term.CONST (\<phi>::object atom formula)"
 
 lemma term_to_obj: "ac_tsubst [] [] (term.CONST x) = x"
   unfolding ac_tsubst_def by simp
 
-(* this is more involved than I thought... *)
 lemma term_to_obj_atom:
   shows "map_atom (ac_tsubst [] []) (map_atom term.CONST x) = x"
 proof (cases x)
-  case (predAtm p xs)
+  case [simp]: (predAtm p xs)
   hence "map_atom (ac_tsubst [] []) (map_atom term.CONST x)
     = predAtm p (map (ac_tsubst [] [] \<circ> term.CONST) xs)"
     by simp
   also have "... = predAtm p xs" using term_to_obj
     by (simp add: map_idI)
-  finally show ?thesis using predAtm by simp
+  finally show ?thesis by simp
 qed (simp add: term_to_obj)
 
 lemma term_to_obj_fmla:
   shows "map_atom_fmla (ac_tsubst [] []) (map_atom_fmla term.CONST F) = F"
   using term_to_obj_atom by (induction F; simp)
 
-lemma resinst_ac_g:
+text \<open> Proving valid_plan_right \<close>
+
+lemma resinst_goal_ac:
   "p3.resolve_instantiate \<pi>\<^sub>g = Ground_Action (goal P) goal_effect"
 proof -
   have "goal_ac term_goal \<in> set (actions D3)" using degoal_dom_sel by simp
@@ -345,70 +321,55 @@ proof -
     (map_atom_fmla (ac_tsubst [] []) term_goal)
     (map_ast_effect (ac_tsubst [] []) goal_effect)"
     using goal_ac_def p3.resolve_instantiate_cond by fastforce
-  moreover have "(map_ast_effect (ac_tsubst [] []) goal_effect) = goal_effect" by simp
-    (* Very simple because there are no parameters, so nothing is actually being mapped.
-       Only the type of an empty list is changed. *)
-  moreover have "map_atom_fmla (ac_tsubst [] []) term_goal = goal P"
-    using term_to_obj_fmla by (simp add: term_goal_def)
-  ultimately show ?thesis by simp
+  thus ?thesis using term_to_obj_fmla term_goal_def by simp
 qed
 
-thm wf_execute   
-lemma "wf_world_model M \<Longrightarrow> wm_basic M"
-  by (meson g_wm_wf p3.wf_fmla_atom_alt p3.wf_world_model_def wm_basic_def)
-
-lemma goal_sem:
+lemma g_goal_sem_right:
   assumes "wf_world_model M" "M \<^sup>c\<TTurnstile>\<^sub>= goal P"
   shows
     "p3.plan_action_enabled \<pi>\<^sub>g M"
     "p3.execute_plan_action \<pi>\<^sub>g M \<^sup>c\<TTurnstile>\<^sub>= goal P3"
 proof -
-  from assms resinst_ac_g wf_pa_g show "p3.plan_action_enabled \<pi>\<^sub>g M"
-    using p3.plan_action_enabled_def by simp
+  from assms show "p3.plan_action_enabled \<pi>\<^sub>g M"
+    using resinst_goal_ac wf_goal_pa p3.plan_action_enabled_def by simp
 
   from assms(1) this
   have basic: "wm_basic (p3.execute_plan_action \<pi>\<^sub>g M)"
     using g_wm_wf p3.wf_execute p3.wf_fmla_atom_alt p3.wf_world_model_def wm_basic_def
     by metis
 
-  from resinst_ac_g have "effect (p3.resolve_instantiate \<pi>\<^sub>g) = goal_effect"
+  from resinst_goal_ac have "effect (p3.resolve_instantiate \<pi>\<^sub>g) = goal_effect"
     by simp
   hence "Atom (predAtm goal_pred []) \<in> p3.execute_plan_action \<pi>\<^sub>g M"
     using p3.execute_plan_action_def by simp
-  hence "valuation (p3.execute_plan_action \<pi>\<^sub>g M) \<Turnstile> goal P3" using degoal_prob_sel(4)
+  hence "valuation (p3.execute_plan_action \<pi>\<^sub>g M) \<Turnstile> goal P3"
     using valuation_def by simp
   with basic show "p3.execute_plan_action \<pi>\<^sub>g M \<^sup>c\<TTurnstile>\<^sub>= goal P3"
     using valuation_iff_close_world by blast
 qed
 
-lemma g_obj_of_type:
-  "is_obj_of_type = p3.is_obj_of_type"
-  unfolding ast_problem.is_obj_of_type_alt ast_domain.is_of_type_def ast_domain.of_type_def
-    ast_domain.subtype_rel_def
-  using g_objT degoal_dom_sel(1) degoal_prob_sel(1) by metis
-
 (* TODO clean up *)
-lemma g_pa_wf_right:
+lemma g_wf_pa_right:
   assumes "wf_plan_action \<pi>"
   shows 
     "resolve_instantiate \<pi> = p3.resolve_instantiate \<pi> \<and> p3.wf_plan_action \<pi>"
 using assms proof (cases \<pi>)
-  case (PAction n args)
+  case [simp]: (PAction n args)
   with assms obtain ac where 1:
     "resolve_action_schema n = Some ac" "ac \<in> set (actions D)" "ac_name ac = n"
     by (meson wf_pa_refs_ac)
-  hence "ac \<in> set (actions D3)" using degoal_dom_sel by simp
+  hence "ac \<in> set (actions D3)" by simp
   with 1 have r: "d3.resolve_action_schema n = Some ac"
     using degoal_prob_sel by (metis p3.res_aux)
   hence g1: "resolve_instantiate \<pi> = p3.resolve_instantiate \<pi>"
-    using degoal_prob_sel 1 PAction by simp
+    using 1 by simp
 
-  from 1 assms have "action_params_match ac args" by (simp add: PAction)
+  from 1 assms have "action_params_match ac args" by simp
   hence "p3.action_params_match ac args"
     unfolding ast_problem.action_params_match_def
     using g_obj_of_type by simp
-  with r have g2: "p3.wf_plan_action \<pi>" using p3.wf_plan_action_simple PAction
-    using degoal_prob_sel(1) PAction by fastforce
+  with r have g2: "p3.wf_plan_action \<pi>"
+    using p3.wf_plan_action_simple PAction by fastforce
 
   from g1 g2 show ?thesis by simp
 qed
@@ -417,151 +378,100 @@ qed
 lemma g_exec_right:
   assumes "wf_plan_action \<pi>"
   shows "execute_plan_action \<pi> M = p3.execute_plan_action \<pi> M"
-  using assms ast_problem.execute_plan_action_def g_pa_wf_right by simp
+  using assms ast_problem.execute_plan_action_def g_wf_pa_right by simp
 
 lemma g_enab_right:
   assumes "wf_plan_action \<pi>"
   shows "plan_action_enabled \<pi> M = p3.plan_action_enabled \<pi> M"
-  using assms g_pa_wf_right ast_problem.plan_action_enabled_def by simp
+  using assms g_wf_pa_right ast_problem.plan_action_enabled_def by simp
 
 lemma g_execs_right:
   assumes "wf_world_model M" "plan_action_path M \<pi>s M'"
   shows "p3.plan_action_path M \<pi>s M'"
   using assms proof (induction \<pi>s arbitrary: M)
 case (Cons p ps)
-  hence 0: "plan_action_enabled p M \<and> plan_action_path (execute_plan_action p M) ps M'"
-    using plan_action_path_Cons by simp
-  with Cons have 1: "p3.plan_action_enabled p M" using g_enab_right
+  hence enab: "plan_action_enabled p M" and path: "plan_action_path (execute_plan_action p M) ps M'"
+    using plan_action_path_Cons by simp_all
+  with Cons have enab3: "p3.plan_action_enabled p M" using g_enab_right
     by (simp add: plan_action_path_def)
-  from wf_execute 0
-  have "wf_world_model (execute_plan_action p M)"
-    by (simp add: Cons.prems(1))
-  note Cons.IH[OF this]
-  with 0 have "p3.plan_action_path (execute_plan_action p M) ps M'" by simp
-  then show ?case
-    using "1" Cons.prems(2) g_exec_right plan_action_path_def by force
+  from Cons enab have "wf_world_model (execute_plan_action p M)"
+    by (simp add: wf_execute)
+  with Cons.IH this path have path2: "p3.plan_action_path (execute_plan_action p M) ps M'" by simp
+  then show ?case using enab enab3 p3.plan_action_path_Cons
+    using g_exec_right plan_action_enabled_def by force
 qed simp
 
-thm plan_action_path_Cons
-
-lemma (in wf_ast_problem) valid_plan_from_Cons[simp]:
-  "valid_plan_from M (\<pi> # \<pi>s)
-    \<longleftrightarrow> valid_plan_from (execute_plan_action \<pi> M) \<pi>s \<and> plan_action_enabled \<pi> M"
-  using valid_plan_from_def by auto
-
-lemma (in wf_ast_problem) valid_plan_from_append:
-  "valid_plan_from M (\<pi>s @ [\<pi>])
-    \<longleftrightarrow> (\<exists>M'. plan_action_path M \<pi>s M' \<and> plan_action_enabled \<pi> M' \<and>
-    execute_plan_action \<pi> M' \<^sup>c\<TTurnstile>\<^sub>= goal P)"
-  using valid_plan_from_def by (induction \<pi>s arbitrary: M; simp)
-
-
-lemma valid_plan_right:
+theorem valid_plan_right:
   assumes "valid_plan \<pi>s"
   shows "p3.valid_plan (\<pi>s @ [\<pi>\<^sub>g])"
 proof -
-
   from assms obtain M where 1: "plan_action_path I \<pi>s M" and 2: "M \<^sup>c\<TTurnstile>\<^sub>= goal P"
     using valid_plan_def valid_plan_from_def by auto
   
   from 1 have wf_m: "wf_world_model M"
     using wf_I wf_plan_action_path by blast
   from 1 have "p3.plan_action_path p3.I \<pi>s M"
-    using ast_problem.I_def g_execs_right degoal_prob_sel(3) wf_I by auto
+    using ast_problem.I_def g_execs_right wf_I by auto
   moreover from 2 wf_m have "p3.plan_action_enabled \<pi>\<^sub>g M"
            "p3.execute_plan_action \<pi>\<^sub>g M \<^sup>c\<TTurnstile>\<^sub>= goal P3"
-    using goal_sem by simp_all
+    using g_goal_sem_right by simp_all
   ultimately show ?thesis
-    using p3.valid_plan_from_append
-    using p3.valid_plan_def by auto
+    using p3.valid_plan_from_snoc p3.valid_plan_def by auto
 qed
 
 (* ------------- left direction ------------- *)
 
-lemma fixes x :: nat assumes "even x" obtains n where "n+n = x"
-proof -
-  from assms obtain n where "n+n = x"
-    by (metis add_self_div_2 div_plus_div_distrib_dvd_right)
-  thus ?thesis ..
-qed
-
 lemma g_ac_split: "ac \<in> set (actions D3) \<longleftrightarrow> ac \<in> set (actions D) \<or> ac = goal_ac term_goal"
   using degoal_dom_sel by auto
 
-lemma (in wf_ast_problem) wf_plan_action_elimd:
-  "wf_plan_action (PAction n args)
-  \<longleftrightarrow> (\<exists>ac. resolve_action_schema n = Some ac \<and>
-    action_params_match ac args)"
-  using wf_plan_action_simple case_optionE by force
+lemma iffOrI: "\<lbrakk>\<lbrakk>A; \<not>C\<rbrakk> \<Longrightarrow> B; B \<Longrightarrow> A; C \<Longrightarrow> A\<rbrakk> \<Longrightarrow> A \<longleftrightarrow> B \<or> C"
+  by blast
 
-thm res_aux
-
-lemma g_wf_pa_split:
+lemma g_wf_pa_left:
   "p3.wf_plan_action \<pi> \<longleftrightarrow> wf_plan_action \<pi> \<or> \<pi> = \<pi>\<^sub>g"
 proof (cases \<pi>)
-  case (PAction n args)
-  note wf_plan_action_elimd
-  have "p3.wf_plan_action (PAction n args) \<longleftrightarrow>
-    (\<exists>ac. p3.resolve_action_schema n = Some ac \<and>
-    p3.action_params_match ac args)" using p3.wf_plan_action_elimd by simp
-  also have "... \<longleftrightarrow> (\<exists>ac. ac \<in> set (actions D3) \<and> ac_name ac = n \<and>
-    p3.action_params_match ac args)" using p3.res_aux
-    by (simp add: degoal_prob_sel(1))
-  also have "... \<longleftrightarrow> (\<exists>ac. (ac \<in> set (actions D) \<or> ac = goal_ac term_goal)
-    \<and> ac_name ac = n \<and> p3.action_params_match ac args)" using g_ac_split by simp
-  also have "... \<longleftrightarrow> (\<exists>ac. (ac \<in> set (actions D) \<and> ac_name ac = n \<and> action_params_match ac args))
-    \<or> (\<exists>ac. ac = goal_ac term_goal \<and> ac_name ac = n \<and> p3.action_params_match ac args)"
-    unfolding ast_problem.action_params_match_def
-    using g_obj_of_type by auto
-  also have 2: "... \<longleftrightarrow> wf_plan_action \<pi> \<or> (\<exists>ac. ac = goal_ac term_goal \<and> ac_name ac = n \<and> p3.action_params_match ac args)"
-    using wf_plan_action_elimd res_aux PAction by simp
-  note a = calculation
+  case [simp]: (PAction n args)
+  show ?thesis proof (rule iffOrI)
+    assume 1: "p3.wf_plan_action \<pi>" and 2: "\<not>\<pi> = \<pi>\<^sub>g"
+    from 1 obtain ac where 3:
+      "d3.resolve_action_schema n = Some ac" "ac \<in> set (actions D3)"
+      "ac_name ac = n" "p3.action_params_match ac args"
+      using p3.wf_pa_refs_ac by auto
 
-  {
-    fix ac
-    assume 1: "ac = goal_ac term_goal \<and> ac_name ac = n \<and> p3.action_params_match ac args"
-    hence "n = goal_ac_name" 
-      using p3.res_aux resolve_ac_g by auto
-    moreover from 1 have "args = []" unfolding goal_ac_def p3.action_params_match_def by auto
-    ultimately have "PAction n args = \<pi>\<^sub>g" by simp
-  }
-  with a show ?thesis
-    using PAction 2 wf_pa_g by force
+    have "ac \<noteq> goal_ac term_goal"
+    proof (rule eq_contr)
+      assume g: "ac = goal_ac term_goal"
+      hence "ac_name ac = goal_ac_name" unfolding goal_ac_def by simp
+      moreover have "args = []" using 3 goal_ac_def p3.action_params_match_def using g by simp
+      ultimately have "\<pi> = \<pi>\<^sub>g" using 3 by simp
+      with 2 show False by simp
+    qed
+
+    hence "ac \<in> set (actions D)" using 3 g_ac_split by simp
+    moreover have "action_params_match ac args"
+      using ast_problem.action_params_match_def g_obj_of_type 3 by simp
+    ultimately show "wf_plan_action \<pi>"
+      using 3 res_aux wf_plan_action_cond
+      by (metis PAction ast_action_schema.exhaust ast_action_schema.sel(1))
+  next
+    assume "wf_plan_action \<pi>" thus "p3.wf_plan_action \<pi>"
+      using g_wf_pa_right by blast
+  next
+    assume "\<pi> = \<pi>\<^sub>g" thus "p3.wf_plan_action \<pi>"
+      using wf_goal_pa by blast
+  qed
 qed
 
 thm entail_adds_irrelevant
-
-lemma (in wf_ast_problem) wf_res_inst:
-  assumes "wf_plan_action \<pi>"
-  shows "wf_ground_action (resolve_instantiate \<pi>)"
-proof (cases \<pi>)
-  case [simp]: (PAction n args)
-  from assms obtain ac where "resolve_action_schema n = Some ac"
-    "action_params_match ac args"
-    using wf_plan_action_elimd by auto
-  moreover from this have "wf_action_schema ac" using res_aux wf_D(7) by simp
-  ultimately show ?thesis using wf_instantiate_action_schema by simp
-qed
-
-lemma
-  "instantiate_action_schema = p3.instantiate_action_schema"
-  by simp
-
+thm wf_ast_problem.wf_resolve_instantiate
 thm wf_pa_refs_ac
+thm g_wf_pa_right
+thm degoal_prob_sel
 
-lemma wf_pa_same_ac:
-  assumes "wf_plan_action (PAction n args)"
-  shows "resolve_action_schema n = d3.resolve_action_schema n"
-proof -
-  from assms obtain ac where "resolve_action_schema n = Some ac \<and> ac \<in> set (actions D) \<and> ac_name ac = n"
-    using wf_pa_refs_ac by metis
-  moreover then have "ac \<in> set (actions D3)" using degoal_dom_sel by simp
-  ultimately show ?thesis using p3.res_aux degoal_prob_sel(1) by metis
-qed
-
-lemma
-  assumes "\<not>M \<^sup>c\<TTurnstile>\<^sub>= goal P3" "wf_plan_action \<pi>"
-  shows "\<not>(execute_plan_action \<pi> M)\<^sup>c\<TTurnstile>\<^sub>= goal P3"
+(* TODO move a lof of goal_pred exclusion logic outside *)
+(* you could use wm_basic in the condition, but then you'd need a version of
+  wf_execute that only cares about preserving wm_basic. *)
+lemma goal_atm_not_wf: "\<not>wf_fmla_atom tyt (Atom (predAtm goal_pred []))"
 proof -
   have "make_unique pred_names ''Goal'' \<notin> set pred_names"
     using made_unique by blast
@@ -569,35 +479,161 @@ proof -
     by auto
   hence "goal_pred \<notin> pred ` set (predicates D)"
     unfolding goal_pred_def using pred_stack by blast
-  note wf_instantiate_action_schema
-  from assms(2) have "wf_ground_action (p3.resolve_instantiate \<pi>)"
-    using wf_res_inst g_pa_wf_right by simp
-  hence "wf_effect objT (effect (p3.resolve_instantiate \<pi>))"
+  hence "\<not>wf_pred_atom tyt (goal_pred, [])"
+    using sig_None wf_pred_atom.simps by (metis option.simps(4))
+  thus ?thesis by simp
+qed
+
+lemma g_goal_unaffected:
+  assumes "\<not>M \<^sup>c\<TTurnstile>\<^sub>= goal P3" "wf_plan_action \<pi>" "p3.wf_world_model M"
+  shows "\<not>(p3.execute_plan_action \<pi> M) \<^sup>c\<TTurnstile>\<^sub>= goal P3"
+proof -
+  let ?goal_atm = "Atom (predAtm goal_pred [])"
+
+  let ?ga = "p3.resolve_instantiate \<pi>"
+
+  from assms(2) have "wf_ground_action ?ga"
+    using g_wf_pa_right wf_resolve_instantiate by simp
+  hence "wf_effect objT (effect ?ga)"
     by (simp add: wf_ground_action_alt)
-  (* formula logic, irrelevants, ... *)
-  oops
+  hence "\<forall>ae \<in> set (adds (effect ?ga)). wf_fmla_atom objT ae"
+    using wf_effect_alt by blast
+  hence notin: "?goal_atm \<notin> set (adds (effect ?ga))"
+    using goal_atm_not_wf by blast
 
-lemma "\<not>p3.I \<^sup>c\<TTurnstile>\<^sub>= goal P3" oops
+  have end_basic: "wm_basic (p3.execute_plan_action \<pi> M)"
+    using assms g_wf_pa_right p3.wf_execute_stronger p3.wf_wm_basic by simp
 
-lemma
-  assumes "\<pi>\<^sub>g \<notin> set (\<pi>s)"
+  (* Todo simplify / export *)
+  from assms have "\<not>(valuation M) \<Turnstile> goal P3"
+    using valuation_iff_close_world p3.wf_wm_basic by blast
+  hence "\<not> (valuation M) (predAtm goal_pred [])"
+    by simp
+  hence "?goal_atm \<notin> M" using valuation_def by simp
+  with notin have "\<not>?goal_atm \<in> p3.execute_plan_action \<pi> M"
+    using p3.execute_plan_action_def p3.apply_effect_alt by simp
+  hence "\<not>(valuation (p3.execute_plan_action \<pi> M)) (predAtm goal_pred [])"
+    using valuation_def by simp
+  hence "\<not>(valuation (p3.execute_plan_action \<pi> M)) \<Turnstile> goal P3"
+    by simp
+  thus ?thesis using assms valuation_iff_close_world
+    end_basic by blast
+qed
+
+lemma g_init_not_sat: "\<not>p3.I \<^sup>c\<TTurnstile>\<^sub>= goal P3"
+proof -
+  have "(Atom (predAtm goal_pred [])) \<notin> I"
+    using wf_P wf_world_model_def goal_atm_not_wf by fastforce
+  hence "\<not>(valuation p3.I) \<Turnstile> goal P3"
+    using valuation_def by simp
+  thus ?thesis using p3.i_basic valuation_iff_close_world by blast
+qed
+
+lemma no_goal_pa_no_sat:
+  assumes "p3.wf_world_model M" "\<not>M \<^sup>c\<TTurnstile>\<^sub>= goal P3" "\<pi>\<^sub>g \<notin> set \<pi>s" "p3.plan_action_path M \<pi>s M'"
+  shows "\<not>M' \<^sup>c\<TTurnstile>\<^sub>= goal P3"
+using assms proof (induction \<pi>s arbitrary: M)
+  case Nil then show ?case
+    using p3.valid_plan_def p3.valid_plan_from_def by auto
+next
+  case (Cons \<pi> \<pi>s)
+  hence "p3.wf_plan_action \<pi>"
+    using p3.plan_action_path_Cons p3.plan_action_enabled_def by blast
+  hence "wf_plan_action \<pi>" using g_wf_pa_left \<open>\<pi>\<^sub>g \<notin> set (\<pi> # \<pi>s)\<close> by auto
+
+  from Cons have 1: "p3.wf_world_model (p3.execute_plan_action \<pi> M)"
+    using p3.wf_execute_stronger \<open>p3.wf_plan_action \<pi>\<close> by simp
+  from Cons have 2: "\<not>(p3.execute_plan_action \<pi> M) \<^sup>c\<TTurnstile>\<^sub>= goal P3"
+    using g_goal_unaffected \<open>wf_plan_action \<pi>\<close> by blast
+  from Cons have 3: "\<pi>\<^sub>g \<notin> set \<pi>s" by simp
+  from Cons have 4: "p3.plan_action_path (p3.execute_plan_action \<pi> M) \<pi>s M'"
+    using p3.plan_action_path_Cons by simp
+
+  from Cons.IH[OF 1 2 3 4] show ?case .
+qed
+
+lemma no_goal_pa_not_valid:
+  assumes "\<pi>\<^sub>g \<notin> set \<pi>s"
   shows "\<not>p3.valid_plan \<pi>s"
-  oops
+proof -
+  have "p3.valid_plan \<pi>s \<longleftrightarrow> (\<exists>M. p3.plan_action_path p3.I \<pi>s M \<and> M \<^sup>c\<TTurnstile>\<^sub>= goal P3)"
+    using p3.valid_plan_def p3.valid_plan_from_def by simp
+  (* with no_goal_pa_no_sat we get
+    p3.plan_action_path p3.I \<pi>s M \<Longrightarrow> \<not>M \<^sup>c\<TTurnstile>\<^sub>= goal P3 *)
+  with assms show ?thesis using g_init_not_sat no_goal_pa_no_sat p3.wf_I by blast
+qed
 
-lemma "x \<in> set xs \<Longrightarrow> (\<exists>ys zs. x \<notin> set ys \<and> ys @ x # zs = xs)"
-  using split_list_first by force
+lemma g_valid_plan_has_ga:
+  "p3.valid_plan \<pi>s \<Longrightarrow> \<pi>\<^sub>g \<in> set \<pi>s"
+  using no_goal_pa_not_valid by auto
 
-lemma
-  assumes "\<pi>\<^sub>g \<notin> set \<pi>s" "p3.plan_action_path M \<pi>s M'"
+lemma g_goal_sem_left:
+  assumes "p3.plan_action_enabled \<pi>\<^sub>g M"
+  shows "M \<^sup>c\<TTurnstile>\<^sub>= goal P"
+using assms p3.plan_action_enabled_def wf_goal_pa
+    resinst_goal_ac by auto
+
+lemma g_exec_left:
+  assumes "p3.wf_plan_action \<pi>" "\<pi> \<noteq> \<pi>\<^sub>g"
+  shows "p3.execute_plan_action \<pi> M = execute_plan_action \<pi> M"
+  using assms g_wf_pa_left g_exec_right by simp
+
+lemma g_enab_left:
+  assumes "p3.wf_plan_action \<pi>" "\<pi> \<noteq> \<pi>\<^sub>g"
+  shows "p3.plan_action_enabled \<pi> M = plan_action_enabled \<pi> M"
+  using assms g_wf_pa_left g_enab_right by simp
+
+lemma g_execs_left:
+  assumes "wf_world_model M" "\<pi>\<^sub>g \<notin> set \<pi>s" "p3.plan_action_path M \<pi>s M'"
   shows "plan_action_path M \<pi>s M'"
-  oops
+using assms proof (induction \<pi>s arbitrary: M)
+  case (Cons \<pi> \<pi>s)
+  hence neq: "\<pi> \<noteq> \<pi>\<^sub>g" and notin: "\<pi>\<^sub>g \<notin> set \<pi>s" by auto
+  from Cons have enab3: "p3.plan_action_enabled \<pi> M" and path3: "p3.plan_action_path (p3.execute_plan_action \<pi> M) \<pi>s M'"
+    by simp_all
+  
+  from enab3 have wf3: "p3.wf_plan_action \<pi>" using p3.plan_action_enabled_def by simp
+  with enab3 have enab: "plan_action_enabled \<pi> M" using neq g_enab_left by simp
+  from path3 wf3 have path2: "p3.plan_action_path (execute_plan_action \<pi> M) \<pi>s M'" using neq g_exec_left by simp
 
-lemma valid_plan_left:
-  assumes "p3.valid_plan \<pi>s'"
-  obtains \<pi>s
-  where "valid_plan \<pi>s"
-  oops
+  from Cons enab have wf_m: "wf_world_model (execute_plan_action \<pi> M)" using wf_execute by simp
 
+  have path: "plan_action_path (execute_plan_action \<pi> M) \<pi>s M'" using Cons.IH[OF wf_m notin path2] .
+
+  from enab path show ?case using plan_action_path_Cons by simp
+qed simp
+
+theorem valid_plan_left:
+  assumes "p3.valid_plan \<pi>s"
+  shows "valid_plan (restore_plan_degoal \<pi>s)"
+proof -
+  let ?ogs = "restore_plan_degoal \<pi>s"
+  from assms obtain ys where
+    restore: "(?ogs @ [\<pi>\<^sub>g]) @ ys = \<pi>s" (* parantheses important for unification with plan_action_path_append_elim *)
+    using g_valid_plan_has_ga sublist_just_until by fastforce
+  from assms obtain M3 where
+    fullpath: "p3.plan_action_path p3.I \<pi>s M3"
+    using p3.valid_plan_def p3.valid_plan_from_def by auto
+  then obtain M2 where
+    path: "p3.plan_action_path p3.I (?ogs @ [\<pi>\<^sub>g]) M2"
+    using p3.plan_action_path_append_elim restore by metis
+  then obtain M1 where
+    sol: "p3.plan_action_path p3.I ?ogs M1" and
+    skip: "p3.plan_action_path M1 [\<pi>\<^sub>g] M2"
+    using p3.plan_action_path_append_elim by blast
+
+  from skip have "p3.plan_action_enabled \<pi>\<^sub>g M1"
+    using plan_action_path_Cons by simp
+  hence sat: "M1 \<^sup>c\<TTurnstile>\<^sub>= goal P"
+    using g_goal_sem_left by simp
+  moreover from sol have "plan_action_path p3.I ?ogs M1"
+    using notin_sublist_until g_execs_left wf_I by fastforce
+  ultimately show ?thesis using valid_plan_def valid_plan_from_def by auto
+qed
+
+theorem degoaled_valid_iff:
+  "(\<exists>\<pi>s. valid_plan \<pi>s) \<longleftrightarrow> (\<exists>\<pi>s. p3.valid_plan \<pi>s)"
+  using valid_plan_left valid_plan_right by auto
 
 end
 
