Tests.thy
@@ -1,16 +1,12 @@
 theory Tests
   imports Main
-    "../LTS-formalization/Datalog/Datalog"
+    (*"../LTS-formalization/Datalog/Datalog"*)
     "AI_Planning_Languages_Semantics.PDDL_STRIPS_Semantics"
     "Show.Show"
-    "AI_Planning_Languages_Semantics.PDDL_STRIPS_Checker"
+    (*"AI_Planning_Languages_Semantics.PDDL_STRIPS_Checker" *)
 begin
 
 (* define single entailment \<TTurnstile>\<^sub>1 :: formula \<Rightarrow> formula \<Rightarrow> bool *)
-
-
-definition fmla_entailment :: "'a formula \<Rightarrow> 'a formula \<Rightarrow> bool" ("(_ \<TTurnstile>\<^sub>1/ _)" [53,53] 53) where
-  "F \<TTurnstile>\<^sub>1 G \<equiv> \<forall>\<A>. \<A> \<Turnstile> F \<longrightarrow> \<A> \<Turnstile> G"
 
 value "shows ''kh'' ''lmao''"
 
